some changes for #92

timesyn/tsynStream.thy
@@ -142,13 +142,13 @@ text {* @{term tsynScanl}: Apply a function elementwise to the input stream. Beh
 definition tsynScanl :: "('b \<Rightarrow> 'a \<Rightarrow> 'b) \<Rightarrow> 'b \<Rightarrow> 'a tsyn stream \<rightarrow> 'b tsyn stream" where
   "tsynScanl f i = tsynScanlExt (\<lambda>a b. (f a b, f a b)) i"
   
-fun tsynDropWhile_h::"('a tsyn \<Rightarrow> bool) \<Rightarrow> 'a tsyn \<Rightarrow> 'a tsyn \<Rightarrow> ('a tsyn \<times> 'a tsyn)" where
+fun tsynDropWhile_h::"('a tsyn \<Rightarrow> bool) \<Rightarrow> bool \<Rightarrow> 'a tsyn \<Rightarrow> ('a tsyn \<times> bool)" where
   "tsynDropWhile_h f x null = (null, x)"|
-  "tsynDropWhile_h f null x = (if f x then (null, null) else (x, x))"|
-  "tsynDropWhile_h f x y = (y, x)"
+  "tsynDropWhile_h f True x = (if f x then (null, True) else (x, False))"|
+  "tsynDropWhile_h f False x = (x, False)"
   
 definition tsynDropWhile :: "('a tsyn \<Rightarrow> bool) \<Rightarrow> 'a tsyn stream \<rightarrow> 'a tsyn stream" where
-  "tsynDropWhile f =  sscanlA (tsynDropWhile_h f) null"
+  "tsynDropWhile f =  sscanlA (tsynDropWhile_h f) True"
 
 (* ----------------------------------------------------------------------- *)
   section {* Fixrec-Definitions on Time-Synchronous Streams *}
@@ -484,17 +484,27 @@ lemma tsynscanl_slen: "#(tsynScanl f i\<cdot>s) = #s"
 (* ----------------------------------------------------------------------- *)
   section {* tsynDropWhile *}
 (* ----------------------------------------------------------------------- *)
-lemma tsyndropwhile_insert:"tsynDropWhile f\<cdot>s = sscanlA (tsynDropWhile_h f) null\<cdot>s "
+
+text {* @{term tsynDropWhile} insertion lemma. *}
+lemma tsyndropwhile_insert:"tsynDropWhile f\<cdot>s = sscanlA (tsynDropWhile_h f) True\<cdot>s "
   by(simp add: tsynDropWhile_def)
     
+text {* @{term tsynDropWhile} is strict. *}
 lemma strict_tsyndropwhile[simp]: "tsynDropWhile f\<cdot>\<epsilon> = \<epsilon>"
   by (simp add: tsyndropwhile_insert)
 
-lemma tsyndropwhile_t[simp]: "f a \<or> a = null \<Longrightarrow> tsynDropWhile f\<cdot>(\<up>a \<bullet> s) = \<up>null \<bullet> tsynDropWhile f\<cdot>s"
+text {* if the head a passes the predicate f, then the head of the result of @{term tsynDropWhile} 
+     will be \<up>null*}
+lemma tsyndropwhile_t: assumes "f a"  shows "tsynDropWhile f\<cdot>(\<up>a \<bullet> s) = \<up>null \<bullet> tsynDropWhile f\<cdot>s"
   apply (simp add: tsyndropwhile_insert)
-  by (metis (no_types, hide_lams) fst_conv snd_conv tsyn.distinct(1) tsynDropWhile_h.elims)
+  by (metis (no_types, hide_lams) assms fst_conv snd_conv tsyn.distinct(1) tsynDropWhile_h.elims)
 
-lemma tsyndropwhile_f_h:"t \<noteq> null \<Longrightarrow> sscanlA (tsynDropWhile_h f) (t)\<cdot>s = s" 
+text {* if the head is null, then the head of the result of @{term tsynDropWhile} will be \<up>null*}    
+lemma tsyndropwhile_null: "tsynDropWhile f\<cdot>(\<up>null \<bullet> s) = \<up>null \<bullet> tsynDropWhile f\<cdot>s"
+  by (simp add: tsyndropwhile_insert)
+
+text {* helplemma for tsyndropwhile_f*}    
+lemma tsyndropwhile_f_h:"t = False \<Longrightarrow> sscanlA (tsynDropWhile_h f) (t)\<cdot>s = s" 
   proof(induction s arbitrary: f t rule: ind)
     case 1
     then show ?case by simp
@@ -503,8 +513,8 @@ lemma tsyndropwhile_f_h:"t \<noteq> null \<Longrightarrow> sscanlA (tsynDropWhil
     then show ?case by simp
   next
     case (3 a s)
-      assume a1:"(\<And>f a. a \<noteq> - \<Longrightarrow> sscanlA (tsynDropWhile_h f) a\<cdot>s = s)"
-      assume a2:"t \<noteq> -"
+      assume a1:"(\<And>f a. a = False \<Longrightarrow> sscanlA (tsynDropWhile_h f) a\<cdot>s = s)"
+      assume a2:"t = False"
       have h0:"sscanlA (tsynDropWhile_h f) t\<cdot>(\<up>a \<bullet> s) =  \<up>(fst (tsynDropWhile_h f t a)) \<bullet> sscanlA (tsynDropWhile_h f) (snd (tsynDropWhile_h f t a))\<cdot>s"
         by simp
       have h1:"\<up>(fst (tsynDropWhile_h f t a)) = \<up>a"
@@ -512,34 +522,61 @@ lemma tsyndropwhile_f_h:"t \<noteq> null \<Longrightarrow> sscanlA (tsynDropWhil
       have h2:"(snd (tsynDropWhile_h f t a)) = t"
         by (metis a2 snd_conv tsynDropWhile_h.elims)
       then show ?case
-        by (simp add: a1 a2 h1) 
+        using a1 a2 h1 by auto
   qed
-    
-lemma tsyndropwhile_f[simp]: "\<not>f a \<and> a \<noteq> null \<Longrightarrow> tsynDropWhile f\<cdot>(\<up>a \<bullet> s) = \<up>a \<bullet> s"
-  apply (simp add: tsyndropwhile_insert,auto)
-  by (metis fst_conv snd_conv tsyn.distinct(1) tsynDropWhile_h.elims tsyndropwhile_f_h)
-
-lemma [simp]: "f a \<or> a = null \<Longrightarrow> tsynDropWhile f\<cdot>(\<up>a) = \<up>null"
-  apply (simp add: tsyndropwhile_insert)
-  by (metis (no_types, hide_lams) fst_conv tsyn.distinct(1) tsynDropWhile_h.elims)
-
-lemma [simp]: "\<not>f a \<and> a \<noteq> Tick\<Longrightarrow> tsynDropWhile f\<cdot>(\<up>a) = \<up>a"
-  by (metis lscons_conv strict_tsyndropwhile sup'_def tsyndropwhile_f tsyndropwhile_t)
-
-lemma tsyndropwhile_idem: "tsynDropWhile f\<cdot>(tsynDropWhile f\<cdot>x) = tsynDropWhile f\<cdot>x"
-  apply (rule ind [of _ x], auto)
-  apply (case_tac "f a",auto)
-  by(case_tac "a = null",auto)
-    
-lemma test_tsyndropwhile: "tsynDropWhile (\<lambda> a. inverseMsg a \<noteq> (2::nat))\<cdot>(<[Msg 1,Msg 1,-,Msg 1, Msg 2, Msg 1]>) = <[-,-,-,-,Msg 2, Msg 1]>"
-  by (simp add: tsyndropwhile_insert)
  
-lemma test2_tsyndropwhile: "tsynDropWhile (\<lambda> a. inverseMsg a \<noteq> (2::nat))\<cdot>(\<up>(Msg 2)\<infinity>) = (\<up>(Msg 2)\<infinity>)"
-  apply(simp add: tsyndropwhile_insert)
-  by (metis (mono_tags, lifting) inverseMsg.simps(2) sinftimes_unfold tsyn.distinct(1) tsynDropWhile_def tsyndropwhile_f)
+text {* if the head a fails the predicate f and is not null, then the head of the result of 
+     @{term tsynDropWhile} will start with \<up>a*}
+lemma tsyndropwhile_f: assumes "\<not>f a" and " a \<noteq> null" shows" tsynDropWhile f\<cdot>(\<up>a \<bullet> s) = \<up>a \<bullet> s"
+  apply (simp add: tsyndropwhile_insert)
+  by (metis assms(1) assms(2) fst_conv snd_conv tsyn.exhaust tsynDropWhile_h.simps(2) tsyndropwhile_f_h)
+    
+text {*  if the only element in a singleton stream passes the predicate f, then 
+     @{term tsynDropWhile} will produce the singleton stream \<up>null *}
+lemma tsyndropwhile_singleton_t: assumes "f a" shows " tsynDropWhile f\<cdot>(\<up>a) = \<up>null"
+  apply (simp add: tsyndropwhile_insert)
+  by (metis (no_types, hide_lams) assms fst_conv tsyn.distinct(1) tsynDropWhile_h.elims)
+ 
+text {*  if the only element in a singleton stream passes is \<up>null, then 
+     @{term tsynDropWhile} will produce the singleton stream \<up>null *}
+lemma tsyndropwhile_singleton_null: "tsynDropWhile f\<cdot>(\<up>null) = \<up>null"
+  by (simp add: tsyndropwhile_insert)
+
+text {*  if the only element in a singleton stream fails the predicate f, then 
+     @{term tsynDropWhile} will be a no-op *}    
+lemma tsyndropwhile_singleton_f: assumes"\<not>f a" shows "tsynDropWhile f\<cdot>(\<up>a) = \<up>a"
+  by (metis assms(1) lscons_conv sup'_def tsyndropwhile_f tsyndropwhile_singleton_null)
   
+text {* @{term tsynDropWhile} is idempotent *}    
+lemma tsyndropwhile_idem: "tsynDropWhile f\<cdot>(tsynDropWhile f\<cdot>x) = tsynDropWhile f\<cdot>x"
+  apply (rule tsyn_ind [of _ x],simp_all)
+  apply (metis tsyndropwhile_f tsyndropwhile_null tsyndropwhile_t)
+  by (simp add: tsyndropwhile_null)
 
+text {* @{term tsynDropWhile} test on finite stream. *}    
+lemma test_tsyndropwhile: "tsynDropWhile (\<lambda> a. \<M>\<inverse> a \<noteq> (2::nat))\<cdot>(<[Msg 1,Msg 1,-,Msg 1, Msg 2, Msg 1]>) = <[-,-,-,-,Msg 2, Msg 1]>"
+  by (simp add: tsyndropwhile_insert)
 
+text {* @{term tsynDropWhile} test on infinite stream. *}
+lemma test2_tsyndropwhile: "tsynDropWhile (\<lambda> a. \<M>\<inverse> a \<noteq> (2::nat))\<cdot>(\<up>(Msg 2)\<infinity>) = (\<up>(Msg 2)\<infinity>)"
+proof(simp add: tsyndropwhile_insert)
+  have f1: "\<And>p t. p (t::nat tsyn) \<or> t = - \<or> sscanlA (tsynDropWhile_h p) True\<cdot>\<up>t\<infinity> = \<up>t\<infinity>"
+    by (metis (no_types) sinftimes_unfold tsynDropWhile_def tsyndropwhile_f)
+  have "\<M>\<inverse> \<M> 2::nat = 2 \<and> \<M> 2::nat \<noteq> -"
+    by (meson inverseMsg.simps(2) tsyn.distinct(1))
+  then show "sscanlA (tsynDropWhile_h (\<lambda>t. (\<M>\<inverse> t::nat) \<noteq> 2)) True\<cdot> \<up>(\<M> 2)\<infinity> = \<up>(\<M> 2)\<infinity>"
+    using f1 by (metis (full_types))
+qed
+  
+text {* @{term tsynDropWhile} test on infinite stream. *}
+lemma test3_tsyndropwhile: "tsynDropWhile (\<lambda> a. \<M>\<inverse> a \<noteq> (2::nat))\<cdot>(\<up>(Msg 1)\<infinity>) = (\<up>(null)\<infinity>)"
+proof(simp add: tsyndropwhile_insert)
+  have "\<And>p t. \<not> p (t::nat tsyn) \<or> sscanlA (tsynDropWhile_h p) True\<cdot>\<up>t\<infinity> = \<up>-\<infinity>"
+    by (metis s2sinftimes sinftimes_unfold tsynDropWhile_def tsyndropwhile_t)
+  then show "sscanlA (tsynDropWhile_h (\<lambda>t. \<M>\<inverse> t \<noteq> 2)) True\<cdot> \<up>(\<M> 1::nat)\<infinity> = \<up>-\<infinity>"
+    by force
+qed
+  
 (* ----------------------------------------------------------------------- *)
   section {* tsynSum - CaseStudy *}
 (* ----------------------------------------------------------------------- *)
